theories/type_systems/stlc_extended/types.v
@@ -320,8 +320,10 @@ Proof.
 Qed.
 
 (** Corollary 15 *)
-Corollary type_safety e1 e2 A:
-  empty |- e1 : A ->
-  rtc contextual_step e1 e2 ->
-  progressive e2.
+Definition safe e :=
+  forall e', rtc contextual_step e e' -> progressive e'.
+
+Corollary type_safety e A:
+  empty |- e : A ->
+  safe e.
 Proof. (* FILL IN HERE (1 LOC proof) *) Admitted.
